chapter02-spec/exercises/exercise02.dfy
@@ -1,34 +1,34 @@
-//#title IsPrime
+//#title IsPrime II
 //#desc Working with an implementation proof
 
-predicate divides(f:nat, i:nat)
-  requires 1<=f
+predicate divides(factor:nat, candidate:nat)
+  requires 1<=factor
 {
-  i % f == 0
+  candidate % factor == 0
 }
 
-predicate IsPrime(i:nat)
+predicate IsPrime(candidate:nat)
 {
-  && 1<i
-  && ( forall f :: 1 < f < i ==> !divides(f, i) )
+  && 1<candidate
+  && ( forall factor :: 1 < factor < candidate ==> !divides(factor, candidate) )
 }
 
 // Convincing the proof to go through requires adding
 // a loop invariant and a triggering assert.
-method test_prime(i:nat) returns (result:bool)
-  requires 1<i
-  ensures result == IsPrime(i)
+method test_prime(candidate:nat) returns (result:bool)
+  requires 1<candidate
+  ensures result == IsPrime(candidate)
 {
   // Fill in the body.
 }
 
 method Main()
 {
-  var a := test_prime(3);
-  assert a;
-  var b := test_prime(4);
+  var isprime3 := test_prime(3);
+  assert isprime3;
+  var isprime4 := test_prime(4);
   assert divides(2, 4);
-  assert !b;
-  var c := test_prime(5);
-  assert c;
+  assert !isprime4;
+  var isprime5 := test_prime(5);
+  assert isprime5;
 }
