chapter01-basics/demos/demo17.dfy
@@ -1,17 +1,17 @@
 // Recursion
 
 // Let's define a function, and export properties of it with an ensures.
-function Evens(x:int) : (s:seq<int>)
-  ensures forall i :: 0<=i<|s| ==> s[i] == 2 * i
+function Evens(count:int) : (outseq:seq<int>)
+  ensures forall idx :: 0<=idx<|outseq| ==> outseq[idx] == 2 * idx
 {
-  if x==0 then [] else Evens(x) + [2 * (x-1)]
+  if count==0 then [] else Evens(count) + [2 * (count-1)]
 }
 
 // Walk through this sequence
 
 Error: cannot prove termination; try supplying a decreases clause
 
-Try adding 'decreases x'.
+Try adding 'decreases count'.
 
 Error: failure to decrease termination measure
 
@@ -19,7 +19,7 @@ Yeah, fix the recursive call.
 
 Error: decreases expression must be bounded below by 0
 
-Hmm. Add 'requires 0 <= x'.
+Hmm. Add 'requires 0 <= count'.
 
 ...and then remove the decreases clause. Now Dafny can guess it!
 
@@ -30,6 +30,6 @@ We want to use assertions, but those are statements, and we're in an
 expression context.
 
 Turns out you can insert assertions before the expression in a function.
-Let's use a var (let) expression to put s in scope.
+Let's use a var (let) expression to put outseq in scope.
 
-Punchline: it doesn't know |s|==x
+Punchline: it doesn't know |outseq|==count
