chapter01-basics/exercises/exercise23.dfy
@@ -8,9 +8,9 @@ include "exercise22.dfy"
 // that one, too). If in doubt about your solution to exercise22, contact
 // an instructor during office hours to make sure you're on the right path.
 
-method FindInBinaryTree(t:Tree, needle:int) returns (b:bool)
-    requires IsSortedTree(t)
-    ensures b <==> needle in TreeAsSequence(t)
+method FindInBinaryTree(tree:Tree, needle:int) returns (issorted:bool)
+    requires IsSortedTree(tree)
+    ensures issorted <==> needle in TreeAsSequence(tree)
 {
     return true;
 }
