chapter02-spec/hints/exercise01_hint.dfy
@@ -1,19 +1,19 @@
 // Here's the body of test_prime. It's correct (you're welcome),
 // but the proof won't go through yet.
-method test_prime(i:nat) returns (result:bool)
-    ensures result == IsPrime(i)
+method test_prime(candidate:nat) returns (result:bool)
+    ensures result == IsPrime(candidate)
 {
-  // Three of these lines are the while version of for(f=0; f<i; f++){}.
-  var f := 2;
-  while (f < i)
+  // Three of these lines are the while version of for(f=0; f<candidate; f++){}.
+  var factor := 2;
+  while (factor < candidate)
   {
-    // If this factor divides i, we've found a counterexample;
-    // i isn't prime.
-    if i % f == 0 {
+    // If this factor divides candidate, we've found a counterexample;
+    // candidate isn't prime.
+    if candidate % factor == 0 {
       return false;
     }
-    f := f + 1;
+    factor := factor + 1;
   }
-  // We tested every possible factor, and none divided i. i is prime.
+  // We tested every possible factor, and none divided candidate. candidate is prime.
   return true;
 }
